lecture7/repeated_squares.dfy
@@ -8,16 +8,16 @@
 
 // Here is the easy recursive version.
 // We want to write a more efficient version.
-function power(x: int, pow: nat): int
+function pow(x: int, exp: nat): int
 {
-  if pow == 0 then 1 else x * power(x, pow - 1)
+  if exp == 0 then 1 else x * pow(x, exp - 1)
 }
 
 // Lemmas
 /* TODO: add lemmas here as needed */
 
-method RepeatedSquare(x: int, pow: nat) returns (y: int)
-  ensures y == power(x, pow)
+method RepeatedSquare(x: int, exp: nat) returns (y: int)
+  ensures y == pow(x, exp)
   // TODO: Uncomment to implement the function
   requires false
 {
