lecture7/advanced.dfy
@@ -1,0 +1,142 @@
+/*
+  Advanced topics that we may not have time to cover in lecture
+
+  - Program termination
+  -
+*/
+
+/*
+  ===== Predicates =====
+*/
+
+// It can be useful to define predicates that can be used in
+// pre/postconditions to make the code more readable.
+
+// A predicate is just a function that returns a boolean.
+// Dafny provides as `predicate` keyword but you can also
+// just use `function`.
+
+// Predicate that holds if a sequence is sorted
+predicate sorted_eq(a: seq<int>, start: int, end: int)
+  requires 0 <= start < end < |a|
+{
+  forall i,j :: start <= i < j < end ==> a[i] <= a[j]
+}
+
+/*
+  ===== Arrays =====
+
+  Arrays are kind of like sequences but they are mutable instead
+  of immutable, so more useful in writing real code.
+  Arrays are not covered on the homework. Using them is more
+  complicated, as we have to worry about what parts of memory
+  are read and written to (`reads` and `modifies` clauses)
+  that can be somewhat subtle.
+
+  Very basic array example: allocating a new array
+
+  (Until now for simplicity we haven't shown any data type
+  allocation, but Dafny allows allocating with the `new` keyword.)
+*/
+
+method Copy(a: array<int>) returns (b: array<int>)
+{
+  b := new int[a.Length];
+  // TODO: copy the array over
+  // This is a HW problem, but on the HW we do it with sequences instead
+}
+
+// Array version of the `sorted` predicate: note the `reads` clause
+// We won't see `reads` a lot in this class, but it will show up on
+// part 2 of the homework.
+predicate sorted_array(a: array<int>, start: int, end: int)
+  reads a
+  requires 0 <= start < end < a.Length
+{
+  forall i,j :: start <= i < j < end ==> a[i] <= a[j]
+}
+
+/*
+  ===== Termination =====
+
+  There's another thing that's implicitly going on with recursion and while loops:
+  program termination.
+
+  Exercise: add a decreases clause to both the fib and ComputeFib
+  functions.
+
+  What does the decreases clause ensure?
+*/
+
+/*
+  ===== Ghost variables and auxiliary state =====
+
+  Sometimes the implementation code is not adequate for dafny to verify
+  postconditions (especially in the presence of loops).
+  Ghost variables are additional state that you can track in the program
+  that is not part of the actual implementation.
+
+  An example of such extra state that might be helpful is a data structure that "logs" some important actions
+  that were done in the loop.
+
+  More generally, Dafny's concept of "ghost" is related to the idea of
+  abstraction.
+  Ghost data are any data that are removed away at runtime,
+  and only present at compile time.
+*/
+
+/*
+  A more philosophical discussion :)
+
+  ===== The limits of verification? =====
+
+  Let's take a step back and consider what we've done so far.
+  - We managed to write a function to calculate Fibonacci numbers and
+    *prove* that it's always correct, on all inputs. Without ever running
+    the code.
+
+  - It was a bit difficult though: we had to come up with a special "loop invariant"
+    and (in theory) a "decreases" clause to make it work,
+    and the code wouldn't verify otherwise.
+    So is this always possible?
+
+  There's sort of an argument for NO and an argument for YES.
+
+  NO: Some of you may have heard that proving general properties
+  about programs is supposed to be impossible!
+  (It's OK if you haven't heard this.) For example,
+  we know that the halting problem is impossible to decide:
+
+    HALT(x) = "Does program x halt?"
+
+  There's no program which decides the above!
+  Yet, Dafny is able to determine not just that all the programs halt,
+  but that they are correct (satisfy the spec) on all inputs.
+  So in Dafny, we could decide the halting problem this way:
+
+    HALT(x): return true;
+
+  Let's take a minute to appreciate what that means: using just some math
+  equations and formulas, and a fancy verification tool (which uses Z3),
+  we know (without running it) that the program will give the correct
+  answer on **all possible inputs.** Not just some particular
+  inputs that we tried. It's a way to completely fool-proof all future uses
+  of the code.
+
+  YES: The surprising thing (at least if you've taken theory of computation)
+  is that in practice, yes, it is almost always possible to prove that
+  programs correct.
+
+  People have even built entire software projects: like cryptographic libraries,
+  operating system kernels, and (famously) an optimizing C compiler (CompCert)
+  entirely in formally verified programming languages.
+    https://sel4.systems/About/
+    https://compcert.org/
+
+  If program termination and correctness is undecidable in general, then how
+  are these projects possible?
+
+  Any ideas? :)
+
+  Answer:
+*/
